\documentclass[]{article}

%opening
\title{}
\author{}

\begin{document}

\maketitle


Возьмем $C_k = \frac{k^k}{(k+1)^{k+1}} = \frac{1}{k}\left(\frac{k}{k+1}\right)^{k+1} \rightarrow 0$, при $k \rightarrow \infty$

Определение метода, сходящегося сверхлинейно:

$||x_{k+1} - x_*|| \le C_k||x_{k} - x_*||$, $C_k \rightarrow 0$ при $k \rightarrow \infty$

В нашем случае $x_* = \lim\limits_{k \to \infty} \frac{1}{k^k} = 0$

$\Rightarrow \frac{1}{(k+1)^{k+1}} \le C_k \frac{1}{k^k} = \frac{k^k}{(k+1)^{k+1}} \frac{1}{k^k} = \frac{1}{(k+1)^{k+1}}$

Получили:
$\frac{1}{(k+1)^{k+1}} \le \frac{1}{(k+1)^{k+1}}$

\end{document}
